fairneris/aneris_lang/lib/serialization/serialization_proof.v
@@ -1,0 +1,694 @@
+From iris.algebra Require Import gmap.
+From fairneris.prelude Require Import misc strings.
+From fairneris.aneris_lang Require Import lang proofmode.
+From fairneris.aneris_lang.lib Require Export serialization_code.
+
+Record serialization := {
+  s_valid_val : val → Prop;
+  s_serializer : serializer;
+  n : nat;
+  m : nat;
+  s_is_ser : val → string → Prop;
+  s_is_ser_valid : ∀ v s, s_is_ser v s -> s_valid_val v;
+  s_ser_spec :
+    ∀ `{anerisG _ _ (live_model_of_user M net_model) Σ} (ip:ip_address) tid ρ f v,
+    s_valid_val v →
+    f ≥ n →
+    {{{ (ip,tid) ↦M {[ ρ := f ]} }}}
+      mkExpr ip (s_serializer.(s_ser) v) @(ip,tid)
+    {{{ (s : string), RET mkVal ip #s; ⌜s_is_ser v s⌝ ∗ (ip,tid) ↦M {[ ρ := f-n ]} }}};
+  s_deser_spec :
+    ∀ `{anerisG _ _ (live_model_of_user M net_model) Σ} ip tid ρ f v s,
+    s_is_ser v s →
+    f ≥ m →
+    {{{ (ip,tid) ↦M {[ ρ := f ]} }}}
+      mkExpr ip (s_serializer.(s_deser) #s) @(ip, tid)
+    {{{ RET mkVal ip v; (ip,tid) ↦M {[ ρ := f-m ]} }}}; }.
+
+Local Hint Resolve  s_is_ser_valid : core.
+
+Class Serializable (s : serialization) (v : val) :=
+  serializable : s_valid_val s v.
+
+Class SerializerOf (ser : serializer) (serion : serialization) :=
+  serializer_of : serion.(s_serializer) = ser.
+
+Definition int_valid_val (v : val) := ∃ (i : Z), v = #i.
+
+Definition int_ser_str (i : Z) : string := StringOfZ i.
+
+Definition int_is_ser (v : val) (s : string) :=
+  ∃ (i : Z), v = #i ∧ s = int_ser_str i.
+
+Lemma int_is_ser_valid (v : val) (s : string) : int_is_ser v s -> int_valid_val v.
+Proof.
+  intros [I [-> _]].
+  eexists _; eauto.
+Qed.
+
+(* Test *)
+Lemma foo 
+  (* Q: Why does this not work? *)
+  (* `{LM:LiveModel aneris_lang (joint_model M Net)} `{!LiveModelEq LM} `{!anerisG LM Σ} *)
+  `{anerisG _ _ (live_model_of_user stenning_model net_model) Σ}
+  ip tid ρ f :
+  f > 40 →
+  {{{ is_node ip ∗ (ip,tid) ↦M {[ ρ := f ]} }}}
+    mkExpr ip ((λ: <>, #()) #()) @ (ip,tid)
+  {{{ v, RET v; True }}}.
+Proof.
+  iIntros (Hf Φ) "[Hnode Hf] HΦ".  
+  wp_pures.
+  iApply wp_value.
+  by iApply "HΦ".
+Qed.
+
+(* TODO: Find a better approach than this. *)
+Lemma has_fuels_mono `{anerisG _ _ (live_model_of_user M net_model) Σ} ζ ρ f1 f2 : 
+  f1 = f2 → ζ ↦M {[ ρ := f1 ]} -∗ ζ ↦M {[ ρ := f2 ]}.
+Proof. by iIntros (->) "$". Qed.
+
+(* TODO: Move this elsewhere *)
+Lemma nat_plus_minus x y z : x - y - z = x - (y + z).
+Proof. lia. Qed.
+
+Tactic Notation "simpl_arith" := repeat rewrite nat_plus_minus.
+Tactic Notation "wp_pures" := (wp_pures; simpl_arith).
+
+Lemma wp_unSOME
+  (* `{LM:LiveModel aneris_lang (joint_model M Net)} `{!LiveModelEq LM} `{!anerisG LM Σ} *)
+  `{anerisG _ _ (live_model_of_user M net_model) Σ}
+  ip tid ρ f v v' :
+  v = SOMEV v' →
+  f > 3 →
+  {{{ (ip,tid) ↦M {[ ρ := f ]} }}}
+    mkExpr ip (unSOME (Val v)) @ (ip,tid)
+  {{{ RET mkVal ip v'; (ip,tid) ↦M {[ ρ := f - 4 ]} }}}.
+Proof.
+  iIntros (-> Hf Φ) "Hf HΦ".
+  wp_lam. wp_match. iApply wp_value. iApply "HΦ".
+  by iApply (has_fuels_mono with "Hf"); lia.
+Qed.
+  
+(* TODO: Generalize to allow multiple roles *)
+Lemma int_ser_spec
+  (* `{LM:LiveModel aneris_lang (joint_model M Net)} `{!LiveModelEq LM} `{!anerisG LM Σ} *)
+  `{anerisG _ _ (live_model_of_user M net_model) Σ}
+  ip tid ρ f v :
+  int_valid_val v →
+  f ≥ 2 →
+  {{{ (ip,tid) ↦M {[ ρ := f ]} }}}
+    mkExpr ip (int_ser v) @ (ip,tid)
+  {{{ (s : string), RET mkVal ip #s; ⌜int_is_ser v s⌝ ∗ (ip,tid) ↦M {[ ρ := f -2 ]} }}}.
+Proof.
+  iIntros ([i ->] Hf Φ) "Hζ HΦ".
+  rewrite /int_ser /int_is_ser.  
+  wp_pures. iApply wp_value. iApply "HΦ"; eauto.
+Qed.
+
+Lemma int_deser_spec
+  (* `{LM:LiveModel aneris_lang (joint_model M Net)} `{!LiveModelEq LM} `{!anerisG LM Σ} *)
+  `{anerisG _ _ (live_model_of_user M net_model) Σ}
+  ip tid ρ f v s :
+  int_is_ser v s →
+  f ≥ 6 →
+  {{{ (ip,tid) ↦M {[ ρ := f ]} }}}
+    mkExpr ip (int_deser #s) @ (ip,tid)
+  {{{ RET mkVal ip v; (ip,tid) ↦M {[ ρ := f - 6 ]} }}}.
+Proof.
+  iIntros ( [i [-> ->]] Hf Φ) "Hf HΦ".
+  rewrite /int_deser /int_is_ser.
+  assert (un_op_eval IntOfString #(StringOfZ i) = Some (InjRV #i)).
+  { rewrite /= ZOfString_inv //=. }
+  wp_pures.
+  iApply (wp_unSOME with "Hf"); [done|lia|].
+  simpl_arith.
+  iIntros "!> Hf". by iApply "HΦ".
+Qed.
+
+Definition int_serialization : serialization :=
+  {| s_valid_val := int_valid_val;
+     s_serializer := int_serializer;
+     s_is_ser := int_is_ser;
+     s_is_ser_valid := int_is_ser_valid;
+     s_ser_spec := @int_ser_spec;
+     s_deser_spec := @int_deser_spec; |}.
+
+Global Instance: ∀ i : Z, Serializable int_serialization #i.
+Proof. intros i; exists i; done. Qed.
+
+Global Instance int_serializer_of : SerializerOf int_serializer int_serialization.
+Proof. done. Qed.
+
+Definition bool_to_int (b : bool) := if b then 1 else 0.
+
+Definition bool_valid_val (v : val) := ∃ (b : bool), v = #b.
+
+Definition bool_ser_str (b : bool) : string :=
+  StringOfZ $ bool_to_int b.
+
+Definition bool_is_ser (v : val) (s : string) :=
+  ∃ (b : bool), v = #b ∧ s = bool_ser_str b.
+
+Lemma bool_is_ser_valid (v : val) (s : string) :
+  bool_is_ser v s -> bool_valid_val v.
+Proof.
+  intros [I [-> _]].
+  eexists _; eauto.
+Qed.
+
+Lemma bool_ser_spec
+  (* `{LM:LiveModel aneris_lang (joint_model M Net)} `{!LiveModelEq LM} `{!anerisG LM Σ} *)
+  `{anerisG _ _ (live_model_of_user stenning_model net_model) Σ}
+  ip tid ρ f v :
+  bool_valid_val v →
+  f ≥ 3 →
+  {{{ (ip,tid) ↦M {[ ρ := f ]} }}}
+    mkExpr ip (bool_ser v) @ (ip,tid)
+  {{{ (s : string), RET mkVal ip #s; ⌜bool_is_ser v s⌝ ∗ (ip,tid) ↦M {[ ρ := f - 3 ]} }}}.
+Proof.
+  iIntros ([b ->] Hf Φ) "Hf HΦ".
+  rewrite /bool_ser /bool_is_ser.
+  destruct b; wp_pures; iApply wp_value; iApply "HΦ"; eauto.
+Qed.
+
+Lemma bool_deser_spec
+  (* `{LM:LiveModel aneris_lang (joint_model M Net)} `{!LiveModelEq LM} `{!anerisG LM Σ} *)
+  `{anerisG _ _ (live_model_of_user stenning_model net_model) Σ}
+  ip tid ρ f v s :
+  bool_is_ser v s →
+  f ≥ 7 →
+  {{{ (ip,tid) ↦M {[ ρ := f ]} }}}
+    mkExpr ip (bool_deser #s) @ (ip,tid)
+  {{{ RET mkVal ip v; (ip,tid) ↦M {[ ρ := f - 7 ]} }}}.
+Proof.
+  iIntros ([b [-> ->]] Hf Φ) "Hf HΦ".
+  rewrite /bool_deser /bool_is_ser. wp_pures.
+  assert (un_op_eval IntOfString #(StringOfZ $ bool_to_int b) =
+          Some (InjRV #(bool_to_int b))).
+  { rewrite /= ZOfString_inv //=. }
+  destruct b; wp_pures; iApply wp_value; by iApply "HΦ".
+Qed.
+
+Definition bool_serialization : serialization :=
+  {| s_valid_val := bool_valid_val;
+     s_serializer := bool_serializer;
+     s_is_ser := bool_is_ser;
+     s_is_ser_valid := bool_is_ser_valid;
+     s_ser_spec := @bool_ser_spec;
+     s_deser_spec := @bool_deser_spec; |}.
+
+Global Instance: ∀ b : bool, Serializable bool_serialization #b.
+Proof. intros b; exists b; done. Qed.
+
+Global Instance bool_serializer_of : SerializerOf bool_serializer bool_serialization.
+Proof. done. Qed.
+
+Definition unit_valid_val (v : val) := v = #().
+
+Definition unit_is_ser (v : val) (s : string) := v = #() ∧ s = "".
+
+Lemma unit_is_ser_valid v s : unit_is_ser v s -> unit_valid_val v.
+Proof.
+  intros [-> _].
+  rewrite /unit_valid_val; done.
+Qed.
+
+Lemma unit_ser_spec
+  (* `{LM:LiveModel aneris_lang (joint_model M Net)} `{!LiveModelEq LM} `{!anerisG LM Σ} *)
+  `{anerisG _ _ (live_model_of_user stenning_model net_model) Σ}
+  ip tid ρ f v :
+  unit_valid_val v →
+  f ≥ 1 →
+  {{{ (ip,tid) ↦M {[ ρ := f ]} }}}
+    mkExpr ip (unit_ser v) @ (ip,tid)
+  {{{ (s : string), RET mkVal ip #s; ⌜unit_is_ser v s⌝ ∗ (ip,tid) ↦M {[ ρ := f - 1 ]} }}}.
+Proof.
+  iIntros (-> Hf Φ) "Hf HΦ".
+  rewrite /unit_ser /unit_is_ser.
+  wp_pures. iApply wp_value. iApply "HΦ"; eauto.
+Qed.
+
+Lemma unit_deser_spec 
+  (* `{LM:LiveModel aneris_lang (joint_model M Net)} `{!LiveModelEq LM} `{!anerisG LM Σ} *)
+  `{anerisG _ _ (live_model_of_user stenning_model net_model) Σ}
+  ip tid ρ f v s :
+  unit_is_ser v s →
+  f ≥ 1 →
+  {{{ (ip,tid) ↦M {[ ρ := f ]} }}}
+    mkExpr ip (unit_deser #s) @ (ip,tid)
+  {{{ RET mkVal ip v; (ip,tid) ↦M {[ ρ := f - 1 ]} }}}.
+Proof.
+  iIntros ([-> ->] Hf Φ) "Hf HΦ".
+  rewrite /unit_deser /unit_is_ser.
+  wp_pures. iApply wp_value. by iApply "HΦ".
+Qed.
+
+Definition unit_serialization : serialization :=
+  {| s_valid_val := unit_valid_val;
+     s_serializer := unit_serializer;
+     s_is_ser := unit_is_ser;
+     s_is_ser_valid := unit_is_ser_valid;
+     s_ser_spec := @unit_ser_spec;
+     s_deser_spec := @unit_deser_spec; |}.
+
+Global Instance: Serializable unit_serialization #().
+Proof. done. Qed.
+
+Global Instance unit_serializer_of : SerializerOf unit_serializer unit_serialization.
+Proof. done. Qed.
+
+Definition string_valid_val (v : val) := ∃ (s : string), v = #s.
+
+Definition string_is_ser (v : val) (s : string) := v = #s.
+
+Lemma string_is_ser_valid v s : string_is_ser v s -> string_valid_val v.
+Proof.
+  intros ->.
+  eexists _; eauto.
+Qed.
+
+Lemma string_ser_spec
+  (* `{LM:LiveModel aneris_lang (joint_model M Net)} `{!LiveModelEq LM} `{!anerisG LM Σ} *)
+  `{anerisG _ _ (live_model_of_user stenning_model net_model) Σ}
+  ip tid ρ f v:
+  string_valid_val v →
+  f ≥ 1 →
+  {{{ (ip,tid) ↦M {[ ρ := f ]} }}}
+    mkExpr ip (string_ser v) @ (ip,tid)
+  {{{ (s : string), RET mkVal ip #s; ⌜string_is_ser v s⌝ ∗ (ip,tid) ↦M {[ ρ := f - 1 ]} }}}.
+Proof.
+  iIntros ([i ->] Hf Φ) "Hf HΦ".
+  rewrite /string_ser /string_is_ser.
+  wp_pures. iApply wp_value. iApply "HΦ"; eauto.
+Qed.
+
+Lemma string_deser_spec
+  (* `{LM:LiveModel aneris_lang (joint_model M Net)} `{!LiveModelEq LM} `{!anerisG LM Σ} *)
+  `{anerisG _ _ (live_model_of_user stenning_model net_model) Σ}
+  ip tid ρ f v s :
+  string_is_ser v s →
+  f ≥ 1 →
+  {{{ (ip,tid) ↦M {[ ρ := f ]} }}}
+    mkExpr ip (string_deser #s) @ (ip,tid)
+  {{{ RET mkVal ip v; (ip,tid) ↦M {[ ρ := f - 1 ]} }}}.
+Proof.
+  iIntros (-> Hf Φ) "Hf HΦ".
+  rewrite /string_deser /string_is_ser.
+  wp_pures. iApply wp_value. iApply "HΦ"; done.
+Qed.
+
+Definition string_serialization : serialization :=
+  {| s_valid_val := string_valid_val;
+     s_serializer := string_serializer;
+     s_is_ser := string_is_ser;
+     s_is_ser_valid := string_is_ser_valid;
+     s_ser_spec := @string_ser_spec;
+     s_deser_spec := @string_deser_spec; |}.
+
+Global Instance: ∀ s : string, Serializable string_serialization #s.
+Proof. intros s; exists s; done. Qed.
+
+Global Instance string_serializer_of : SerializerOf string_serializer string_serialization.
+Proof. done. Qed.
+
+Section prod_serialization.
+
+  Context (A B : serialization).
+
+  Definition prod_valid_val (v : val) :=
+    ∃ v1 v2, v = (v1, v2)%V ∧ s_valid_val A v1 ∧ s_valid_val B v2.
+
+  Definition prod_ser_str (s1 s2 : string) :=
+    StringOfZ (String.length s1) +:+ "_" +:+ s1 +:+ s2.
+
+  Definition prod_is_ser (v : val) (s : string) :=
+    ∃ v1 v2 s1 s2,
+      v = (v1, v2)%V ∧ s_is_ser A v1 s1 ∧ s_is_ser B v2 s2 ∧
+      s = prod_ser_str s1 s2.
+
+  Lemma prod_is_ser_valid v s : prod_is_ser v s -> prod_valid_val v.
+  Proof.
+    intros [v1 [v2 [s1 [s2 [-> [Hl [Hr _]]]]]]].
+    rewrite /prod_valid_val; eauto 10.
+  Qed.
+
+  Lemma prod_ser_spec
+    (* `{LM:LiveModel aneris_lang (joint_model M Net)} `{!LiveModelEq LM} `{!anerisG LM Σ} *)
+    `{anerisG _ _ (live_model_of_user stenning_model net_model) Σ}
+    ip tid ρ f v :
+    prod_valid_val v →
+    f ≥ 12 + n A + n B →
+    {{{ (ip,tid) ↦M {[ ρ := f ]} }}}
+      mkExpr ip (prod_ser A.(s_serializer).(s_ser) B.(s_serializer).(s_ser) v) @ (ip,tid)
+    {{{ (s : string), RET mkVal ip #s; ⌜prod_is_ser v s⌝ ∗ (ip,tid) ↦M {[ ρ := f - (12 + n A + n B) ]} }}}.
+  Proof.
+    iIntros ((v1&v2&->&?&?) Hf Φ) "Hf HΦ".
+    rewrite /prod_ser /prod_is_ser.
+    wp_pures.
+    wp_bind (s_ser (s_serializer A) v1).
+    iApply (s_ser_spec A with "Hf"); [done|lia|].
+    iIntros (s1) "!> [%HA Hf]".
+    wp_pures. 
+    wp_bind (s_ser (s_serializer B) v2).
+    iApply (s_ser_spec B with "Hf"); [done|lia|].
+    iIntros (s2) "!> [%HB Hf]".
+    wp_pures. iApply wp_value. iApply "HΦ".
+    iSplitR.
+    - iPureIntro. exists v1, v2, s1, s2; split_and!; auto.
+    - iApply (has_fuels_mono with "Hf"). lia.
+  Qed.
+
+  Lemma prod_deser_spec
+    (* `{LM:LiveModel aneris_lang (joint_model M Net)} `{!LiveModelEq LM} `{!anerisG LM Σ} *)
+    `{anerisG _ _ (live_model_of_user stenning_model net_model) Σ}
+    ip tid ρ f v s :
+    prod_is_ser v s →
+    f ≥ 31 + m A + m B →
+    {{{ (ip,tid) ↦M {[ ρ := f ]} }}}
+      mkExpr ip (prod_deser A.(s_serializer).(s_deser) B.(s_serializer).(s_deser) #s)
+      @ (ip,tid)
+    {{{ RET mkVal ip v; (ip,tid) ↦M {[ ρ := f - (31 + m A + m B) ]} }}}.
+  Proof.
+    iIntros ((v1 & v2 & s1 & s2 & -> & Hv1 & Hv2 & ->) Hf Φ) "Hf HΦ".
+    rewrite /prod_deser /prod_is_ser /prod_ser_str.
+    wp_pures.
+    wp_find_from; first by split_and!; [|by apply nat_Z_eq; first lia].
+    erewrite (index_0_append_char ); auto; last first.
+    { apply valid_tag_stringOfZ. }
+    wp_pures.
+    wp_substring; first by split_and!; [|by apply nat_Z_eq; first lia|done].
+    rewrite substring_0_length_append.
+    wp_pure _.
+    { rewrite /= ZOfString_inv //. }
+    wp_pures. wp_bind (unSOME _).
+    iApply (wp_unSOME with "Hf"); [done|lia|].
+    iIntros "!> Hf"; simpl.
+    wp_pures.
+    wp_substring; first by split_and!; [|by apply nat_Z_eq; first lia|done].
+    replace (Z.to_nat (Z.add (Z.of_nat
+                                (String.length
+                                   (StringOfZ (Z.of_nat (String.length s1)))))
+                             1%Z)) with
+        (String.length (StringOfZ (Z.of_nat (String.length s1))) + 1)%nat by lia.
+    rewrite substring_add_length_app /= substring_0_length_append.
+    wp_pures.
+    rewrite !length_app /=.
+    match goal with
+    | |- context [Substring _ _ ?X] =>
+      replace X with (Val #(String.length s2)); last first
+    end.
+    { repeat f_equal; lia. }
+    wp_substring; first by split_and!; [|by apply nat_Z_eq; first lia|done].
+    match goal with
+    | |- context [substring ?X _ _] =>
+      replace X with (String.length
+                        (StringOfZ (Z.of_nat (String.length s1))) + 1 +
+                      String.length s1)%nat by lia
+    end.
+    rewrite -Nat.add_assoc substring_add_length_app /= substring_length_append.
+    wp_pures.
+    wp_bind (s_deser _ _).
+    iApply (s_deser_spec A with "Hf"); [done|lia|].
+    iIntros "!> Hf".
+    wp_pures.
+    wp_bind (s_deser _ _).
+    iApply (s_deser_spec B with "Hf"); [done|lia|].
+    iIntros "!> Hf".
+    simpl_arith.
+    wp_pures. iApply wp_value. iApply "HΦ".
+    iApply (has_fuels_mono with "Hf"); lia.
+  Qed.
+
+  Definition prod_serialization : serialization :=
+    {| s_valid_val := prod_valid_val;
+       s_serializer := prod_serializer A.(s_serializer) B.(s_serializer);
+       s_is_ser := prod_is_ser;
+       s_is_ser_valid := prod_is_ser_valid;
+       s_ser_spec := @prod_ser_spec;
+       s_deser_spec := @prod_deser_spec; |}.
+
+  Global Instance:
+    ∀ v1 v2, Serializable A v1 → Serializable B v2 →
+             Serializable prod_serialization (v1, v2).
+  Proof. rewrite /Serializable /= /prod_valid_val /=; eauto. Qed.
+
+  Global Instance prod_serializer_of serA serB :
+    SerializerOf serA A → SerializerOf serB B →
+    SerializerOf (prod_serializer serA serB) (prod_serialization).
+  Proof.
+    intros H1 H2.
+    rewrite /SerializerOf.
+    rewrite /SerializerOf in H1.
+    rewrite /SerializerOf in H2.
+    subst. done.
+  Qed.
+
+End prod_serialization.
+
+(* Section sum_serialization. *)
+
+(*   Context (A B : serialization). *)
+
+(*   Definition sum_valid_val (v : val) := *)
+(*     ∃ w, (v = InjLV w ∧ s_valid_val A w) ∨ *)
+(*          (v = InjRV w ∧ s_valid_val B w). *)
+
+(*   Definition inl_ser_str (s : string) := "L_" +:+ s. *)
+(*   Definition inr_ser_str (s : string) := "R_" +:+ s. *)
+
+(*   Definition sum_is_ser (v : val) (s : string) := *)
+(*     ∃ w s', *)
+(*       (v = InjLV w ∧ s_is_ser A w s' ∧ s = inl_ser_str s') ∨ *)
+(*       (v = InjRV w ∧ s_is_ser B w s' ∧ s = inr_ser_str s'). *)
+
+(*   Lemma sum_is_ser_valid v s : sum_is_ser v s -> sum_valid_val v. *)
+(*   Proof. *)
+(*     intros [w [s' [(? & ? & _) | (? & ? & ?)]]]; *)
+(*       rewrite /sum_valid_val; eauto 10. *)
+(*   Qed. *)
+
+(*   Lemma sum_ser_spec `{!anerisG Mdl Σ} ip v: *)
+(*     {{{ ⌜sum_valid_val v⌝ }}} *)
+(*       sum_ser A.(s_serializer).(s_ser) B.(s_serializer).(s_ser) v @[ip] *)
+(*     {{{ (s : string), RET #s; ⌜sum_is_ser v s⌝ }}}. *)
+(*   Proof. *)
+(*     iIntros (Φ [w Hw]) "HΦ". *)
+(*     rewrite /sum_ser /sum_is_ser. *)
+(*     destruct Hw as [[-> Hw]|[-> Hw]]; wp_pures. *)
+(*     - wp_apply (s_ser_spec A); first done. *)
+(*       iIntros (s Hs); simpl. *)
+(*       wp_pures. *)
+(*       iApply "HΦ"; eauto 10. *)
+(*     - wp_apply (s_ser_spec B); first done. *)
+(*       iIntros (s Hs); simpl. *)
+(*       wp_pures. *)
+(*       iApply "HΦ"; eauto 10. *)
+(*   Qed. *)
+
+(*   Lemma sum_deser_spec `{!anerisG Mdl Σ} ip v s: *)
+(*     {{{ ⌜sum_is_ser v s⌝ }}} *)
+(*       sum_deser A.(s_serializer).(s_deser) B.(s_serializer).(s_deser) #s @[ip] *)
+(*     {{{ RET v; True }}}. *)
+(*   Proof. *)
+(*     iIntros (Φ (w & s' & Hw)) "HΦ". *)
+(*     rewrite /sum_deser /sum_is_ser. *)
+(*     wp_pures. *)
+(*     destruct Hw as [(->&?&->)|(->&?&->)]. *)
+(*     - wp_substring; *)
+(*         first by split_and!; *)
+(*               [|by apply nat_Z_eq; first lia|by apply nat_Z_eq; first lia]. *)
+(*       rewrite (substring_0_length_append "L_"). *)
+(*       wp_pures. *)
+(*       wp_substring; *)
+(*         first by split_and!; *)
+(*               [|by apply nat_Z_eq; first lia|by apply nat_Z_eq; first lia]. *)
+(*       rewrite (substring_add_length_app _ _ "L_") /=. *)
+(*       replace (Z.to_nat (S (S (String.length s')) - 2)) with *)
+(*           (String.length s') by lia. *)
+(*       rewrite substring_0_length. *)
+(*       wp_pures. *)
+(*       wp_apply (s_deser_spec A); first done. *)
+(*       iIntros "_". *)
+(*       wp_pures. *)
+(*       iApply "HΦ"; done. *)
+(*     - wp_substring; *)
+(*         first by split_and!; *)
+(*               [|by apply nat_Z_eq; first lia|by apply nat_Z_eq; first lia]. *)
+(*       rewrite (substring_0_length_append "R_"). *)
+(*       wp_pures. *)
+(*       wp_substring; *)
+(*         first by split_and!; *)
+(*               [|by apply nat_Z_eq; first lia|by apply nat_Z_eq; first lia]. *)
+(*       rewrite (substring_add_length_app _ _ "R_") /=. *)
+(*       replace (Z.to_nat (S (S (String.length s')) - 2)) with *)
+(*           (String.length s') by lia. *)
+(*       rewrite substring_0_length. *)
+(*       wp_pures. *)
+(*       wp_apply (s_deser_spec B); first done. *)
+(*       iIntros "_". *)
+(*       wp_pures. *)
+(*       iApply "HΦ"; done. *)
+(*   Qed. *)
+
+(*   Definition sum_serialization : serialization := *)
+(*     {| s_valid_val := sum_valid_val; *)
+(*        s_serializer := sum_serializer A.(s_serializer) B.(s_serializer); *)
+(*        s_is_ser := sum_is_ser; *)
+(*        s_is_ser_valid := sum_is_ser_valid; *)
+(*        s_ser_spec := @sum_ser_spec; *)
+(*        s_deser_spec := @sum_deser_spec; |}. *)
+
+(*   Global Instance : *)
+(*     ∀ v, Serializable A v → Serializable sum_serialization (InjLV v). *)
+(*   Proof. rewrite /Serializable /= /sum_valid_val /=; eauto. Qed. *)
+
+(*   Global Instance : *)
+(*     ∀ v, Serializable B v → Serializable sum_serialization (InjRV v). *)
+(*   Proof. rewrite /Serializable /= /sum_valid_val /=; eauto. Qed. *)
+
+(*   Global Instance sum_serializer_of serA serB : *)
+(*     SerializerOf serA A → SerializerOf serB B → *)
+(*     SerializerOf (sum_serializer serA serB) (sum_serialization). *)
+(*   Proof. *)
+(*     intros H1 H2. *)
+(*     rewrite /SerializerOf. *)
+(*     rewrite /SerializerOf in H1. *)
+(*     rewrite /SerializerOf in H2. *)
+(*     subst. done. *)
+(*   Qed. *)
+
+(* End sum_serialization. *)
+
+(* (* *) *)
+(* (* Option serialization can be defined using sum_serialization. *) *)
+(* (* However, from the point of view of translation from OCaml to AnerisLang, *) *)
+(* (* it was more convenient to define option serialization separately. *) *)
+(* (* Indeed, in OCaml sources, option expressions (None and Some e) and sum type *) *)
+(* (* expresions (InjL e1 and InjR e2) are kept separately - to make programming a *) *)
+(* (* little bit more natural while in AnerisLang - which is untyped - optional *) *)
+(* (* expressions are a particular type of sum expressions. *) *)
+(* (* That is, translation itself takes care of translating native Ocaml *) *)
+(* (* optional expressions, values and patterns into AnerisLang sum expressions. *) *)
+(* (* *) *)
+(* Section option_serialization. *)
+
+(*   Context (T : serialization). *)
+
+
+(*   Definition option_valid_val (v : val) := *)
+(*     (∃ w, v = InjRV w ∧ s_valid_val T w) ∨ *)
+(*     (v = InjLV #()). *)
+
+(*   Definition option_None_ser_str := inl_ser_str "". *)
+(*   Definition option_Some_ser_str (s : string) := inr_ser_str s. *)
+
+(*   Definition option_is_ser (v : val) (s : string) := *)
+(*     (v = InjLV #() ∧ s = option_None_ser_str) ∨ *)
+(*     (∃ w s', v = InjRV w ∧ s_is_ser T w s' ∧ s = option_Some_ser_str s'). *)
+
+(*   Lemma option_is_ser_valid v s : option_is_ser v s -> option_valid_val v. *)
+(*   Proof. *)
+(*     intros [[-> _] | [? [? [? [? ?]]]]]; rewrite /option_valid_val; eauto 10. *)
+(*   Qed. *)
+
+(*   Lemma option_ser_spec `{!anerisG Mdl Σ} ip v: *)
+(*     {{{ ⌜option_valid_val v⌝ }}} *)
+(*       option_ser T.(s_serializer).(s_ser) v @[ip] *)
+(*     {{{ (s : string), RET #s; ⌜option_is_ser v s⌝ }}}. *)
+(*   Proof. *)
+(*     iIntros (Φ Hw) "HΦ". *)
+(*     rewrite /option_ser /s_ser /s_serializer /option_is_ser. *)
+(*     destruct Hw as [[w (-> & Hw)]|Hw]; wp_pures. *)
+(*     - wp_apply (s_ser_spec T); first done. *)
+(*       iIntros (s Hs); simpl. *)
+(*       wp_pures. *)
+(*       iApply "HΦ"; eauto 10. *)
+(*     - rewrite Hw. wp_pures. *)
+(*       iApply "HΦ". eauto. *)
+(*   Qed. *)
+
+(*   Lemma option_deser_spec `{!anerisG Mdl Σ} ip v s: *)
+(*     {{{ ⌜option_is_ser v s⌝ }}} *)
+(*       option_deser T.(s_serializer).(s_deser) #s @[ip] *)
+(*     {{{ RET v; True }}}. *)
+(*   Proof. *)
+(*     iIntros (Φ Hw) "HΦ". *)
+(*     rewrite /option_deser /option_is_ser /s_ser /s_serializer. *)
+(*     wp_pures. *)
+(*     destruct Hw as [(-> & ->) |(w & (s' & (-> & ? & ->)))]. *)
+(*     - wp_substring; *)
+(*         first by split_and!; *)
+(*                           [|by apply nat_Z_eq; first lia|by apply nat_Z_eq; first lia]. *)
+(*       wp_pures. *)
+(*       wp_substring; *)
+(*         first by split_and!; *)
+(*               [|by apply nat_Z_eq; first lia|by apply nat_Z_eq; first lia]. *)
+(*       rewrite (substring_add_length_app _ _ "L_") /=. *)
+(*       wp_pures. by iApply "HΦ". *)
+(*     - wp_substring; *)
+(*         first by split_and!; *)
+(*               [|by apply nat_Z_eq; first lia|by apply nat_Z_eq; first lia]. *)
+(*       rewrite (substring_0_length_append "R_"). *)
+(*       wp_pures. *)
+(*       wp_substring; *)
+(*         first by split_and!; *)
+(*               [|by apply nat_Z_eq; first lia|by apply nat_Z_eq; first lia]. *)
+(*       rewrite (substring_add_length_app _ _ "R_") /=. *)
+(*       replace (Z.to_nat (S (S (String.length s')) - 2)) with *)
+(*           (String.length s') by lia. *)
+(*       rewrite substring_0_length. *)
+(*       wp_pures. *)
+(*       wp_apply (s_deser_spec T); first done. *)
+(*       iIntros "_". *)
+(*       wp_pures. *)
+(*       iApply "HΦ"; done. *)
+(*   Qed. *)
+
+(*   Definition option_serialization : serialization := *)
+(*     {| s_valid_val := option_valid_val; *)
+(*        s_serializer := option_serializer T.(s_serializer); *)
+(*        s_is_ser := option_is_ser; *)
+(*        s_is_ser_valid := option_is_ser_valid; *)
+(*        s_ser_spec := @option_ser_spec; *)
+(*        s_deser_spec := @option_deser_spec; |}. *)
+
+(*   Global Instance: *)
+(*     ∀ v, Serializable T v → Serializable option_serialization (SOMEV v). *)
+(*   Proof. *)
+(*     rewrite /Serializable /= /option_valid_val /=; eauto. *)
+(*   Qed. *)
+
+(*   Global Instance: Serializable option_serialization (NONEV). *)
+(*   Proof. rewrite /Serializable /= /option_valid_val /option_valid_val /=. by right. Qed. *)
+
+(*   Global Instance option_serializer_of serT : *)
+(*     SerializerOf serT T → *)
+(*     SerializerOf (option_serializer serT) (option_serialization). *)
+(*   Proof. *)
+(*     intros H1. *)
+(*     rewrite /SerializerOf. *)
+(*     rewrite /SerializerOf in H1. *)
+(*     subst. done. *)
+(*   Qed. *)
+
+(* End option_serialization. *)
+
+(* Recursively destructs the definition of the argument hypothesis of the shape *)
+(*    [H : *_is_ser] *)
+Ltac destruct_is_ser H :=
+  match type of H with
+  | s_is_ser _ _ _ => simpl in H; destruct_is_ser H
+  | int_is_ser _ _ => destruct H as (?&?&?)
+  | unit_is_ser _ _ => destruct H as [? ?]
+  | prod_is_ser _ _ _ _ =>
+    destruct H as (?&?&?&?&?& ?Hp1 & ?Hp2 &?);
+    destruct_is_ser Hp1; destruct_is_ser Hp2
+  (* | sum_is_ser _ _ _ _ => *)
+  (*   destruct H as (?&?& [(? & ?Hl & ?)|(? & ?Hr &?)]); *)
+  (*   [destruct_is_ser Hl | destruct_is_ser Hr] *)
+  (* | option_is_ser _ _ _ => *)
+  (*   destruct H as (?&?& [(? & ?Hl & ?)|(? & ?Hr & ?)]); *)
+  (*   [destruct_is_ser Hl | destruct_is_ser Hr] *)
+  | _ => idtac
+  end; simplify_eq.
